Begin to work with concrete networks, which can be programmatically manipulated.

Circuits/Interp.lean
@@ -1,26 +1,26 @@
-import «Circuits».Network
+import «Circuits».Network.Abstract
 import «Circuits».Circuit
 
-def Network.toCircuit (interp : (c : Component) → Circuit (Terminal c)) (net : Network Component Terminal α) : Circuit α :=
+def Network.Abstract.toCircuit (interp : (c : Component) → Circuit (Terminal c)) (net : Network.Abstract Component Terminal α) : Circuit α :=
   Circuit.map net.wiring $
   Circuit.merge (ι := net.Node) (α := Terminal ∘ net.component) $
   fun node => interp (net.component node)
 
 
 
-theorem Interp.single : (Network.single c).toCircuit interp = interp c := by
-  simp only [Network.toCircuit, Network.single, Circuit.merge_unit, <-Circuit.comp_map, 𝔽.Cospan.ofEquiv]
+theorem Interp.single : (Network.Abstract.single c).toCircuit interp = interp c := by
+  simp only [Network.Abstract.toCircuit, Network.Abstract.single, Circuit.merge_unit, <-Circuit.comp_map, 𝔽.Cospan.ofEquiv]
   rw [Circuit.map.congr (g := 𝔽.Cospan.id), Circuit.id_map]
   exact (𝔽.Cospan.comp_ofFwd _ _).symm
 
-theorem Interp.map (f : 𝔽.Cospan α β) (net : Network Component Terminal α) : (net.map f).toCircuit interp = (net.toCircuit interp).map f := by
-  simp only [Network.toCircuit, Network.single, Network.map, <-Circuit.comp_map]
+theorem Interp.map (f : 𝔽.Cospan α β) (net : Network.Abstract Component Terminal α) : (net.map f).toCircuit interp = (net.toCircuit interp).map f := by
+  simp only [Network.Abstract.toCircuit, Network.Abstract.single, Network.Abstract.map, <-Circuit.comp_map]
 
-theorem Interp.merge {ι : 𝔽} {α : ι → 𝔽} (net : (i : ι) → Network Component Terminal (α i)) :
-  (Network.merge ι α net).toCircuit interp = Circuit.merge ι (fun i => (net i).toCircuit interp)
+theorem Interp.merge {ι : 𝔽} {α : ι → 𝔽} (net : (i : ι) → Network.Abstract Component Terminal (α i)) :
+  (Network.Abstract.merge ι α net).toCircuit interp = Circuit.merge ι (fun i => (net i).toCircuit interp)
 := by
-  simp only [Network.toCircuit, Network.single, Circuit.merge_map]
-  simp only [Network.merge, Circuit.merge_sigma, <-Circuit.comp_map]
+  simp only [Network.Abstract.toCircuit, Network.Abstract.single, Circuit.merge_map]
+  simp only [Network.Abstract.merge, Circuit.merge_sigma, <-Circuit.comp_map]
   apply Circuit.map.congr
   calc 𝔽.Cospan.comp _ (𝔽.Cospan.comp _ (𝔽.Cospan.merge fun i => (net i).wiring))
     𝔽.Cospan.Equiv _ _ := (𝔽.Cospan.comp.assoc _ _ _).symm
