Circuits/Network/Concrete.lean
@@ -1,0 +1,19 @@
+import «Circuits».Utils
+
+namespace Network
+
+structure Concrete (Component : Type) where
+  Wire : ℕ
+  nodes : Array (Component × Array ℕ)
+  terminals : Array ℕ
+def Concrete.single (c : Component) (Terminal : ℕ) : Concrete Component where
+  Wire := Terminal
+  nodes := Array.mk [⟨c, Array.ofFn (n := Terminal) fun i => i⟩]
+  terminals := Array.ofFn (n := Terminal) fun i => i
+def Concrete.merge (nets : Array (Concrete Component)) : Concrete Component :=
+  let offsets := Array.mk ((nets.toList.map Concrete.Wire).scanl Nat.add 0)
+  let offset {k : ℕ} (i : Fin k) (n : ℕ) := offsets[i]! + n
+  { Wire := offsets[nets.size]!
+  , nodes := nets.concatMap fun net => net.nodes.map $ Prod.map id fun arr => arr.mapIdx offset
+  , terminals := nets.concatMap fun net => net.terminals.mapIdx offset
+  }
