Circuits/Network/Properties.lean
@@ -1,0 +1,55 @@
+import Mathlib.Data.FinEnum
+import «Circuits».Network.Concrete
+import «Circuits».Network.Abstract
+
+namespace Network
+
+structure Represents
+  {Component : Type} [Inhabited Component]
+  {Terminal : Component → Type} [∀ c, FinEnum (Terminal c)]
+  {α : Type} [FinEnum α]
+  (conc : Concrete Component)
+  (abs : Abstract Component (fun c => Terminal c) α)
+where
+  node : abs.Node → ℕ
+  component (n : abs.Node) : abs.component n = (conc.nodes.get! (node n)).1
+  wiring_center : abs.wiring.center → ℕ
+  wiring_bwd (a : α) : wiring_center (abs.wiring.bwd a) = conc.terminals.get! (FinEnum.equiv a)
+  wiring_fwd (n : abs.Node) (t : Terminal (abs.component n)) :
+    wiring_center (abs.wiring.fwd ⟨n,t⟩) = (conc.nodes.get! (node n)).2.get! (FinEnum.equiv t)
+
+structure Bundled
+  (Component : Type) [Inhabited Component]
+  (Terminal : Component → Type) [∀ c, FinEnum (Terminal c)]
+  (α : Type) [FinEnum α]
+where
+  concrete : Concrete Component
+  abstract : Abstract Component (fun c => Terminal c) α
+  repr : Represents concrete abstract
+
+lemma Array.getD_eq_getElem {α : Type u} (l : Array α) (d : α) {n : ℕ} (hn : n < l.size) : l.getD n d = l[n] := by
+  simp only [Array.getD, Array.get_eq_getElem]; split <;> rfl
+
+def Bundled.single
+  {Component : Type} [Inhabited Component]
+  {Terminal : Component → Type} [∀ c, FinEnum (Terminal c)]
+  (c : Component) :
+  Bundled Component Terminal (Terminal c)
+where
+  concrete := Concrete.single c (FinEnum.card (Terminal c))
+  abstract := Abstract.single c
+  repr.node := fun () => 0
+  repr.component := fun () => rfl
+  repr.wiring_center := by
+    change Terminal c → ℕ
+    exact fun x => ↑(FinEnum.equiv x)
+  repr.wiring_fwd := fun () x => by
+    change (FinEnum.equiv x).val = (Array.ofFn fun i => ↑i).get! (FinEnum.equiv x).val
+    rw [Array.get!, Array.getD_eq_getElem, Array.getElem_ofFn]
+    simp only [Array.size_ofFn]
+    apply Fin.isLt
+  repr.wiring_bwd x := by
+    change (FinEnum.equiv x).val = (Array.ofFn fun i => ↑i).get! (FinEnum.equiv x).val
+    rw [Array.get!, Array.getD_eq_getElem, Array.getElem_ofFn]
+    simp only [Array.size_ofFn]
+    apply Fin.isLt
